# baseURI: http://linked.data.gov.au/def/auorg
# imports: http://www.w3.org/2006/time
# imports: http://www.w3.org/ns/org#
# imports: http://www.w3.org/ns/time/gregorian
# imports: http://xmlns.com/foaf/0.1/

@prefix : <http://linked.data.gov.au/def/auorg/> .
@prefix agrif: <http://reference.data.gov.au/def/ont/agrif#> .
@prefix dc: <http://purl.org/dc/elements/1.1/> .
@prefix dct: <http://purl.org/dc/terms/> .
@prefix dcterms: <http://purl.org/dc/terms/> .
@prefix gnaf: <http://gnafld.net/def/gnaf#> .
@prefix org: <http://www.w3.org/ns/org#> .
@prefix owl: <http://www.w3.org/2002/07/owl#> .
@prefix rdf: <http://www.w3.org/1999/02/22-rdf-syntax-ns#> .
@prefix rdfs: <http://www.w3.org/2000/01/rdf-schema#> .
@prefix skos: <http://www.w3.org/2004/02/skos/core#> .
@prefix time: <http://www.w3.org/2006/time> .
@prefix vann: <http://purl.org/vocab/vann/> .
@prefix xml: <http://www.w3.org/XML/1998/namespace> .
@prefix xsd: <http://www.w3.org/2001/XMLSchema#> .

gnaf:Address
  rdf:type owl:Class ;
.
<http://linked.data.gov.au/def/auorg>
  rdf:type owl:Ontology ;
  dc:contributor "Simon J.D. Cox" ;
  dc:creator "Nicholas J. Car" ;
  dc:publisher "CSIRO" ;
  dcterms:contributor <https://orcid.org/0000-0002-3884-3420> ;
  dcterms:created "2018-05-21"^^xsd:date ;
  dcterms:creator <http://orcid.org/0000-0002-8742-7730> ;
  dcterms:modified "2018-09-12"^^xsd:date ;
  dcterms:publisher <http://www.csiro.au> ;
  vann:preferredNamespacePrefix "auorg" ;
  rdfs:comment """The purpose of this ontology is to allow for the Semantic Web representation of Australian Federal Government Entities (organisations), their subcomponents and people related to them with particular roles.

This ontology specialises the W3C's recommended Organization Ontology to model Entities. Its specialised classes and properties have been initially informed by the Australian government's online organisations directory, https://www.directory.gov.au. This includes particular types of organisation found in Australian Federal government such as a 'Board', 'Government Entity' and so on.

Further specialisation and extension is likely as this ontology is developed to cover the conceptual space of systems that are important for Australian government structure, such as the Administrative Arrangement Orders that alter Entities.

This ontology is incomplete as of v0.6 and is currently for demo purposes only."""@en ;
  rdfs:label "AU Org Ontology"@en ;
  rdfs:seeAlso "The GitHub repository containing addition documentation: http://github.com/CSIRO-enviro-informatics/auorg-ont/"@en ;
  owl:imports <http://www.w3.org/2006/time> ;
  owl:imports org: ;
  owl:imports <http://www.w3.org/ns/time/gregorian> ;
  owl:imports <http://xmlns.com/foaf/0.1/> ;
  owl:versionIRI : ;
  owl:versionInfo "0.7 reduced in scope removing Appropriations Framework concepts" ;
  owl:versionInfo "Beta version"@en ;
.
:ABS
  rdf:type :Agency ;
  :levelOfGovernment :Federal ;
  rdfs:label "Australian Bureau of Statistics" ;
  org:linkedTo :CommonwealthOfAustralia ;
.
:AbolitionEvent
  rdf:type owl:Class ;
  rdfs:comment """An Abolition Event abolishes an Entity. It may also be a creation event in that it could also create an entity.

This Change Event subclass is disjoint with Modification Event."""@en ;
  rdfs:label "Abolition Event"@en ;
  rdfs:subClassOf org:ChangeEvent ;
  owl:disjointWith :ModificationEvent ;
.
:Agency
  rdf:type owl:Class ;
  rdfs:comment "The Governor-General appoints ministers, establishes departments of state and agencies, and allocates responsibility among ministers through an Administrative Arrangements Order (AAO)."@en ;
  rdfs:isDefinedBy <https://www.australia.gov.au/about-government/departments-and-agencies> ;
  rdfs:label "Government Agency" ;
  rdfs:subClassOf :Entity ;
  rdfs:subClassOf [
      rdf:type owl:Restriction ;
      owl:onProperty org:linkedTo ;
      owl:someValuesFrom :Jurisdiction ;
    ] ;
  rdfs:subClassOf [
      rdf:type owl:Restriction ;
      owl:onProperty org:purpose ;
      owl:someValuesFrom agrif:Function ;
    ] ;
  skos:altLabel "Departments of State" ;
.
:AustralianCapitalTerritory
  rdf:type :Jurisdiction ;
  rdf:type owl:NamedIndividual ;
  :levelOfGovernment :State ;
  rdfs:label "Australian Capital Territory" ;
  org:subOrganizationOf :CommonwealthOfAustralia ;
.
:BoM
  rdf:type :Agency ;
  :levelOfGovernment :Federal ;
  rdfs:label "Bureau of Meteorology" ;
  org:linkedTo :CommonwealthOfAustralia ;
.
:Board
  rdf:type owl:Class ;
  rdfs:comment "An Australian Government Board"@en ;
  rdfs:label "Board"@en ;
  rdfs:subClassOf org:FormalOrganization ;
.
:CEO
  rdf:type org:Role ;
  rdfs:label "Chief Executive Officer" ;
.
:CEO-CSIRO
  rdf:type org:Post ;
  rdfs:label "Chief Executive of CSIRO" ;
  org:postIn :CSIRO ;
  org:role :CEO ;
.
:CEO-GA
  rdf:type org:Post ;
  rdfs:label "Chief Executive Officer of GA" ;
  org:postIn :GA ;
  org:role :CEO ;
.
:CSIRO
  rdf:type :CorporateEntity ;
  :levelOfGovernment :Federal ;
  rdfs:label "Commonwealth Scientific and Industrial Research Organisation" ;
  org:linkedTo :CommonwealthOfAustralia ;
.
:CommonwealthOfAustralia
  rdf:type :Jurisdiction ;
  rdf:type owl:NamedIndividual ;
  :levelOfGovernment :Federal ;
  rdfs:comment """The Commonwealth of Australia.

Australia's formal name is the Commonwealth of Australia. Australia is both a representative democracy and a constitutional monarchy with Queen Elizabeth II as Australia's head of state."""@en ;
  rdfs:isDefinedBy <https://www.australia.gov.au/about-government/how-government-works> ;
  rdfs:label "Commonwealth of Australia"@en ;
  org:hasSubOrganization :AustralianCapitalTerritory ;
  org:hasSubOrganization :NewSouthWales ;
  org:hasSubOrganization :NorthernTerritory ;
  org:hasSubOrganization :Queensland ;
  org:hasSubOrganization :SouthAustralia ;
  org:hasSubOrganization :Tasmania ;
  org:hasSubOrganization :Victoria ;
  org:hasSubOrganization :WesternAustralia ;
.
:CorporateEntity
  rdf:type owl:Class ;
  rdfs:comment "The Governor-General appoints ministers, establishes departments of state and agencies, and allocates responsibility among ministers through an Administrative Arrangements Order (AAO)."@en ;
  rdfs:isDefinedBy <https://www.australia.gov.au/about-government/departments-and-agencies> ;
  rdfs:label "Government Corporate Entity" ;
  rdfs:subClassOf :Entity ;
  rdfs:subClassOf [
      rdf:type owl:Restriction ;
      owl:onProperty org:linkedTo ;
      owl:someValuesFrom :Jurisdiction ;
    ] ;
  rdfs:subClassOf [
      rdf:type owl:Restriction ;
      owl:onProperty org:purpose ;
      owl:someValuesFrom agrif:Function ;
    ] ;
.
:CreationEvent
  rdf:type owl:Class ;
  rdfs:comment """A Creation Event is one that creates a Government Entity. It could also be an Abolition Event when the same even both abolishes and creates Entities. 

This Change Event subclass is disjoint with Modification Event."""@en ;
  rdfs:label "Creation Event"@en ;
  rdfs:subClassOf org:ChangeEvent ;
  owl:disjointWith :ModificationEvent ;
.
:Department
  rdf:type owl:Class ;
  rdfs:comment "a Government Department" ;
  rdfs:label "Government Department" ;
  rdfs:subClassOf :Entity ;
  rdfs:subClassOf org:OrganizationalUnit ;
  rdfs:subClassOf [
      rdf:type owl:Restriction ;
      owl:onProperty org:purpose ;
      owl:someValuesFrom agrif:Function ;
    ] ;
  rdfs:subClassOf [
      rdf:type owl:Restriction ;
      owl:onProperty org:unitOf ;
      owl:someValuesFrom :Jurisdiction ;
    ] ;
.
:DepartmentSecretary
  rdf:type owl:NamedIndividual ;
  rdf:type org:Role ;
  rdfs:comment "Public servant who is head of a department" ;
  rdfs:label "Department Secretary" ;
.
:Director
  rdf:type org:Role ;
  rdfs:label "Director" ;
.
:DoEE
  rdf:type :Department ;
  :levelOfGovernment :Federal ;
  rdfs:label "Department of the Environment and Energy" ;
  org:linkedTo :CommonwealthOfAustralia ;
.
:Entity
  rdf:type owl:Class ;
  rdfs:comment "Government entity, any kind, any level of government" ;
  rdfs:label "Government Entity" ;
  rdfs:subClassOf org:Organization ;
  rdfs:subClassOf [
      rdf:type owl:Restriction ;
      owl:cardinality "1"^^xsd:nonNegativeInteger ;
      owl:onProperty :levelOfGovernment ;
    ] ;
.
:Federal
  rdf:type owl:NamedIndividual ;
  rdf:type skos:Concept ;
  rdfs:comment "Federal government, of the Commonwealth of Australia, as outlined in the Australian Constritution" ;
  rdfs:label "Federal" ;
.
:Finance
  rdf:type :Department ;
  :levelOfGovernment :Federal ;
  rdfs:label "Department of Finance" ;
  org:linkedTo :CommonwealthOfAustralia ;
.
:GA
  rdf:type :Agency ;
  :levelOfGovernment :Federal ;
  rdfs:label "Geoscience Australia" ;
  org:linkedTo :CommonwealthOfAustralia ;
.
:GG
  rdf:type org:Post ;
  rdfs:label "Governor General of Australia" ;
  org:postIn :CommonwealthOfAustralia ;
  org:role :GovernorGeneral ;
.
:GovernorGeneral
  rdf:type owl:NamedIndividual ;
  rdf:type org:Role ;
  rdfs:comment """The representative of the Australian monarch in the Commonwealth of Australia.

The Governor-General is appointed by the Australian monarch on the advice of the Prime Minister of Australia. The Governor-General has formal presidency over the Federal Executive Council and is Commander-in-Chief of the Australian Defence Force""" ;
  rdfs:label "Governor-General"@en ;
.
:Jurisdiction
  rdf:type owl:Class ;
  rdfs:comment "This applies to the top/autonomous government entity - e.g. one for each national, state, local government jurisdiction" ;
  rdfs:label "Government or Jurisdiction" ;
  rdfs:subClassOf :Entity ;
.
:Local
  rdf:type owl:NamedIndividual ;
  rdf:type skos:Concept ;
  rdfs:label "Local government" ;
.
:Minister
  rdf:type owl:NamedIndividual ;
  rdf:type org:Role ;
  rdfs:comment "Political head of department" ;
  rdfs:label "Minister" ;
.
:MinisterEnergy
  rdf:type org:Post ;
  rdfs:label "Minister of Energy" ;
  org:postIn :DoEE ;
  org:role :Minister ;
.
:MinisterEnvironment
  rdf:type org:Post ;
  rdfs:label "Minister of Environment" ;
  org:postIn :DoEE ;
  org:role :Minister ;
.
:MinisterFinance
  rdf:type org:Post ;
  rdfs:label "Minister of Finance" ;
  org:postIn :Finance ;
  org:role :Minister ;
.
:ModificationEvent
  rdf:type owl:Class ;
  rdfs:comment "An event that modifies an existing Entity but doesn't create or abolish any Entities."@en ;
  rdfs:label "Modification Event"@en ;
  rdfs:subClassOf org:ChangeEvent ;
.
:NAA
  rdf:type :Agency ;
  :levelOfGovernment :Federal ;
  rdfs:label "National Archives of Australia" ;
  org:linkedTo :CommonwealthOfAustralia ;
.
:NewSouthWales
  rdf:type :Jurisdiction ;
  rdf:type owl:NamedIndividual ;
  :levelOfGovernment :State ;
  rdfs:label "New South Wales" ;
  org:subOrganizationOf :CommonwealthOfAustralia ;
.
:NonBoard
  rdf:type owl:Class ;
  rdfs:comment "An Australian Government non-board entity"@en ;
  rdfs:label "Non-Board"@en ;
  rdfs:subClassOf org:FormalOrganization ;
.
:NorthernTerritory
  rdf:type :Jurisdiction ;
  rdf:type owl:NamedIndividual ;
  :levelOfGovernment :State ;
  rdfs:label "Northern Territory" ;
  org:subOrganizationOf :CommonwealthOfAustralia ;
.
:Queensland
  rdf:type :Jurisdiction ;
  rdf:type owl:NamedIndividual ;
  :levelOfGovernment :State ;
  rdfs:label "Queensland" ;
  org:subOrganizationOf :CommonwealthOfAustralia ;
.
:SingleExecutiveRole
  rdf:type owl:Class ;
  rdfs:comment "A single executive (Senior Executive Service in the Australian Public Service) role"@en ;
  rdfs:label "Single Executive Role"@en ;
  rdfs:subClassOf org:Post ;
.
:SouthAustralia
  rdf:type :Jurisdiction ;
  rdf:type owl:NamedIndividual ;
  :levelOfGovernment :State ;
  rdfs:label "South Australia" ;
  org:subOrganizationOf :CommonwealthOfAustralia ;
.
:State
  rdf:type owl:NamedIndividual ;
  rdf:type skos:Concept ;
  rdfs:label "State or Territory" ;
.
:Tasmania
  rdf:type :Jurisdiction ;
  rdf:type owl:NamedIndividual ;
  :levelOfGovernment :State ;
  rdfs:label "Tasmania" ;
  org:subOrganizationOf :CommonwealthOfAustralia ;
.
:Victoria
  rdf:type :Jurisdiction ;
  rdf:type owl:NamedIndividual ;
  :levelOfGovernment :State ;
  rdfs:label "Victoria" ;
  org:subOrganizationOf :CommonwealthOfAustralia ;
.
:WesternAustralia
  rdf:type :Jurisdiction ;
  rdf:type owl:NamedIndividual ;
  :levelOfGovernment :State ;
  rdfs:label "Western Australia" ;
  org:subOrganizationOf :CommonwealthOfAustralia ;
.
:hasABN
  rdf:type owl:DatatypeProperty ;
  rdfs:comment "org:identifier is a sub-property of skos:notation, which is a owl:DatatypeProperty, i.e. a literal. Could be constrained to be a string with the pattern 'NN NNN NNN NNN` to match ABN structure" ;
  rdfs:label "has ABN" ;
  rdfs:range xsd:integer ;
  rdfs:subPropertyOf org:identifier ;
.
:hasAverageStaffingLevel
  rdf:type owl:DatatypeProperty ;
  rdfs:comment "has an average annual staffing level of (no. of people)"@en ;
  rdfs:label "has average staffing level" ;
  rdfs:range xsd:integer ;
.
:hasStreetAddress
  rdf:type owl:ObjectProperty ;
  rdfs:comment "has a GNAF address of"@en ;
  rdfs:label "has street address" ;
  rdfs:range gnaf:Address ;
  rdfs:subPropertyOf org:hasSite ;
.
:levelOfGovernment
  rdf:type owl:ObjectProperty ;
  rdfs:comment "level of government (Federal, State, Local)" ;
  rdfs:domain :Jurisdiction ;
  rdfs:label "level of government" ;
  rdfs:subPropertyOf org:classification ;
.
agrif:Function
  rdf:type owl:Class ;
.
agrif:associatedFunction
  rdf:type owl:ObjectProperty ;
  rdfs:comment "A relation that associates a Function to an Entity, Event or Activity." ;
  rdfs:domain :Entity ;
  rdfs:isDefinedBy <http://reference.data.gov.au/def/ont/agrif> ;
  rdfs:label "associated function" ;
  rdfs:range agrif:Function ;
  rdfs:subPropertyOf org:classification ;
.
skos:altLabel
  rdf:type owl:AnnotationProperty ;
.
org:purpose
  rdf:type owl:ObjectProperty ;
.
