@prefix : <http://linked.data.gov.au/def/auorg#> .
@prefix dc: <http://purl.org/dc/elements/1.1/> .
@prefix dct: <http://purl.org/dc/terms/> .
@prefix org: <http://www.w3.org/ns/org#> .
@prefix owl: <http://www.w3.org/2002/07/owl#> .
@prefix rdf: <http://www.w3.org/1999/02/22-rdf-syntax-ns#> .
@prefix xml: <http://www.w3.org/XML/1998/namespace> .
@prefix xsd: <http://www.w3.org/2001/XMLSchema#> .
@prefix gnaf: <http://gnafld.net/def/gnaf#> .
@prefix rdfs: <http://www.w3.org/2000/01/rdf-schema#> .
@base <http://linked.data.gov.au/def/auorg> .

<http://linked.data.gov.au/def/auorg> rdf:type owl:Ontology ;
                                       owl:versionIRI <http://linked.data.gov.au/def/auorg/0.6> ;
                                       owl:imports <http://www.w3.org/ns/time/gregorian> ,
                                                   <http://www.w3.org/2006/time> ,
                                                   org: ;
                                       dc:creator "Nicholas J. Car" ;
                                       rdfs:label "AU Org Ontology"@en ;
                                       dct:modified "2018-05-21"^^xsd:date ,
                                                    "2018-09-05"^^xsd:date ;
                                       dct:publisher <http://www.csiro.au> ;
                                       dc:publisher "CSIRO" ;
                                       owl:versionInfo "0.6 has been reviewed and enhanced by Simon Cox" ;
                                       dct:contributor <https://orcid.org/0000-0002-3884-3420> ;
                                       owl:versionInfo "Beta version"@en ;
                                       dct:creator <http://orcid.org/0000-0002-8742-7730> ;
                                       dct:created "2018-05-21"^^xsd:date ;
                                       dc:contributor "Simon J.D. Cox" ;
                                       rdfs:seeAlso "The GitHub repository containing addition documentation: http://github.com/CSIRO-enviro-informatics/auorg-ont/"@en ;
                                       rdfs:comment """The purpose of this ontology is to allow for the Semantic Web representation of Australian Federal Government Entities (organisations), their subcomponents and people related to them with particular roles.

This ontology specialises the W3C's recommended Organization Ontology to model Entities. Its specialised classes and properties have been initially informed by the Australian government's online organisations directory, https://www.directory.gov.au. This includes particular types of organisation found in Australian Federal government such as a 'Board', 'Government Entity' and so on.

Further specialisation and extension is likely as this ontology is developed to cover the conceptual space of systems that are important for Australian government structure, such as the Administrative Arrangement Orders that alter Entities.

This ontology is incomplete as of v0.6 and is currently for demo purposes only."""@en .

#################################################################
#    Annotation properties
#################################################################

###  http://purl.org/dc/elements/1.1/contributor
dc:contributor dct:description "Examples of a Contributor include a person, an organization, or a service. Typically, the name of a Contributor should be used to indicate the entity."@en ;
               dct:hasVersion <http://dublincore.org/usage/terms/history/#contributor-006> ;
               dct:issued "1999-07-02"^^xsd:date ;
               dct:modified "2008-01-14"^^xsd:date ;
               rdfs:comment "An entity responsible for making contributions to the resource."@en ;
               rdfs:isDefinedBy dc: ;
               rdfs:label "Contributor"@en ;
               <http://www.w3.org/2004/02/skos/core#note> "A second property with the same name as this property has been declared in the dcterms: namespace (http://purl.org/dc/terms/).  See the Introduction to the document \"DCMI Metadata Terms\" (http://dublincore.org/documents/dcmi-terms/) for an explanation."@en .


###  http://purl.org/dc/elements/1.1/creator
dc:creator dct:description "Examples of a Creator include a person, an organization, or a service. Typically, the name of a Creator should be used to indicate the entity."@en ;
           dct:hasVersion <http://dublincore.org/usage/terms/history/#creator-006> ;
           dct:issued "1999-07-02"^^xsd:date ;
           dct:modified "2008-01-14"^^xsd:date ;
           rdfs:comment "An entity primarily responsible for making the resource."@en ;
           rdfs:isDefinedBy dc: ;
           rdfs:label "Creator"@en ;
           <http://www.w3.org/2004/02/skos/core#note> "A second property with the same name as this property has been declared in the dcterms: namespace (http://purl.org/dc/terms/).  See the Introduction to the document \"DCMI Metadata Terms\" (http://dublincore.org/documents/dcmi-terms/) for an explanation."@en .


###  http://purl.org/dc/elements/1.1/publisher
dc:publisher dct:description "Examples of a Publisher include a person, an organization, or a service. Typically, the name of a Publisher should be used to indicate the entity."@en ;
             dct:hasVersion <http://dublincore.org/usage/terms/history/#publisher-006> ;
             dct:issued "1999-07-02"^^xsd:date ;
             dct:modified "2008-01-14"^^xsd:date ;
             rdfs:comment "An entity responsible for making the resource available."@en ;
             rdfs:isDefinedBy dc: ;
             rdfs:label "Publisher"@en ;
             <http://www.w3.org/2004/02/skos/core#note> "A second property with the same name as this property has been declared in the dcterms: namespace (http://purl.org/dc/terms/).  See the Introduction to the document \"DCMI Metadata Terms\" (http://dublincore.org/documents/dcmi-terms/) for an explanation."@en .


###  http://purl.org/dc/terms/description
dct:description rdf:type owl:AnnotationProperty .


###  http://purl.org/dc/terms/hasVersion
dct:hasVersion rdf:type owl:AnnotationProperty .


###  http://purl.org/dc/terms/issued
dct:issued rdf:type owl:AnnotationProperty .


###  http://purl.org/dc/terms/modified
dct:modified rdf:type owl:AnnotationProperty .


###  http://purl.org/dc/terms/publisher
dct:publisher rdf:type owl:AnnotationProperty .


###  http://purl.org/dc/terms/title
dct:title rdf:type owl:AnnotationProperty .


#################################################################
#    Object Properties
#################################################################

###  http://linked.data.gov.au/def/auorg#budgetDuration
:budgetDuration rdf:type owl:ObjectProperty ;
                rdfs:domain :BudgetItem ;
                rdfs:range <http://www.w3.org/2006/time#TemporalDuration> ;
                rdfs:label "duration of interval over which budget applies" .


###  http://linked.data.gov.au/def/auorg#budgetInterval
:budgetInterval rdf:type owl:ObjectProperty ;
                rdfs:domain :BudgetItem ;
                rdfs:range <http://www.w3.org/2006/time#ProperInterval> ;
                rdfs:label "interval over which budget applies" .


###  http://linked.data.gov.au/def/auorg#budgetPurpose
:budgetPurpose rdf:type owl:ObjectProperty ;
               rdfs:domain :BudgetItem ;
               rdfs:range :Function ;
               rdfs:label "purpose for which budget is allocated" .


###  http://linked.data.gov.au/def/auorg#budgetQuantity
:budgetQuantity rdf:type owl:ObjectProperty ;
                rdfs:domain :BudgetItem ;
                rdfs:range :SumOfMoney ;
                rdfs:label "budget quantity" .


###  http://linked.data.gov.au/def/auorg#budgetSource
:budgetSource rdf:type owl:ObjectProperty ;
              rdfs:domain :BudgetItem ;
              rdfs:range <http://xmlns.com/foaf/0.1/Agent> ;
              rdfs:label "source of budget" .


###  http://linked.data.gov.au/def/auorg#hasAppropriations
:hasAppropriations rdf:type owl:ObjectProperty ;
                   rdfs:subPropertyOf :hasBudgetItem ;
                   rdfs:range :Appropriations ;
                   rdfs:comment "Has a current annual budgetary appropriation amount in Australian Dollars" ;
                   rdfs:label "Annual appropriation budget (AUD)" .


###  http://linked.data.gov.au/def/auorg#hasBudgetItem
:hasBudgetItem rdf:type owl:ObjectProperty ;
               rdfs:domain org:Organization ;
               rdfs:range :BudgetItem ;
               rdfs:label "budget item" .


###  http://linked.data.gov.au/def/auorg#hasStreetAddress
:hasStreetAddress rdf:type owl:ObjectProperty ;
                  rdfs:subPropertyOf org:hasSite ;
                  rdfs:range gnaf:Address ;
                  rdfs:comment "Has a GNAF address of"@en ;
                  rdfs:label "has street address"@en .


###  http://linked.data.gov.au/def/auorg#inPortfolio
:inPortfolio rdf:type owl:ObjectProperty ;
             rdfs:subPropertyOf org:subOrganizationOf ;
             rdfs:range :Portfolio ;
             rdfs:comment "is within a particular government Portfolio"@en ;
             rdfs:label "in portfolio"@en .


###  http://linked.data.gov.au/def/auorg#levelOfGovernment
:levelOfGovernment rdf:type owl:ObjectProperty ;
                   rdfs:subPropertyOf org:classification ;
                   rdfs:domain :Government ;
                   rdfs:label "level of government (Federal, State, Local)" .


###  http://www.w3.org/ns/org#purpose
org:purpose rdf:type owl:ObjectProperty .


#################################################################
#    Data properties
#################################################################

###  http://linked.data.gov.au/def/auorg#hasABN
:hasABN rdf:type owl:DatatypeProperty ;
        rdfs:subPropertyOf org:identifier ;
        rdfs:range xsd:integer ;
        rdfs:comment "org:identifier is a sub-property of skos:notation, which is a owl:DatatypeProperty, i.e. a literal. Could be constrained to be a string with the pattern 'NN NNN NNN NNN` to match ABN structure" .


###  http://linked.data.gov.au/def/auorg#hasAverageStaffingLevel
:hasAverageStaffingLevel rdf:type owl:DatatypeProperty ;
                         rdfs:range xsd:integer ;
                         rdfs:comment "Has an average annual staffig level of (no. of people)"@en ;
                         rdfs:label "has average staffing level"@en .


###  http://linked.data.gov.au/def/auorg#moneyAmount
:moneyAmount rdf:type owl:DatatypeProperty ;
             rdfs:domain :SumOfMoney ;
             rdfs:range xsd:decimal ;
             rdfs:label "Money amount" .


###  http://linked.data.gov.au/def/auorg#moneyCurrency
:moneyCurrency rdf:type owl:DatatypeProperty ;
               rdfs:domain :SumOfMoney ;
               rdfs:range xsd:string ;
               rdfs:label "Money currency - ISO 4217 code" .


#################################################################
#    Classes
#################################################################

###  http://gnafld.net/def/gnaf#Address
gnaf:Address rdf:type owl:Class ;
             rdfs:subClassOf org:Site ;
             rdfs:comment "An Address object, defined by the GNAF ontology and supplied by the GNAF dataset only."@en ;
             rdfs:label "Address"@en .


###  http://linked.data.gov.au/def/auorg#Appropriations
:Appropriations rdf:type owl:Class ;
                rdfs:subClassOf :BudgetItem ,
                                [ rdf:type owl:Restriction ;
                                  owl:onProperty :budgetQuantity ;
                                  owl:allValuesFrom :AustralianDollars
                                ] ,
                                [ rdf:type owl:Restriction ;
                                  owl:onProperty :budgetDuration ;
                                  owl:hasValue <http://www.w3.org/2006/time#unitYear>
                                ] ,
                                [ rdf:type owl:Restriction ;
                                  owl:onProperty :budgetSource ;
                                  owl:hasValue :CommonwealthOfAustralia
                                ] ;
                rdfs:label "Appropriations budget (annualized)" .


###  http://linked.data.gov.au/def/auorg#AustralianDollars
:AustralianDollars rdf:type owl:Class ;
                   rdfs:subClassOf :SumOfMoney ,
                                   [ rdf:type owl:Restriction ;
                                     owl:onProperty :moneyAmount ;
                                     owl:allValuesFrom xsd:integer
                                   ] ,
                                   [ rdf:type owl:Restriction ;
                                     owl:onProperty :moneyCurrency ;
                                     owl:hasValue "AUD"
                                   ] ;
                   rdfs:comment "Sum of money in whole Australian Dollars"@en ;
                   rdfs:label "Australian Dollars"@en .


###  http://linked.data.gov.au/def/auorg#Board
:Board rdf:type owl:Class ;
       rdfs:subClassOf org:FormalOrganization ;
       rdfs:comment "An Australian Government Board"@en ;
       rdfs:label "Board"@en .


###  http://linked.data.gov.au/def/auorg#BudgetItem
:BudgetItem rdf:type owl:Class ;
            rdfs:subClassOf [ rdf:type owl:Restriction ;
                              owl:onProperty :budgetPurpose ;
                              owl:minCardinality "1"^^xsd:nonNegativeInteger
                            ] ,
                            [ rdf:type owl:Restriction ;
                              owl:onProperty :budgetSource ;
                              owl:minCardinality "1"^^xsd:nonNegativeInteger
                            ] ,
                            [ rdf:type owl:Restriction ;
                              owl:onProperty :budgetDuration ;
                              owl:cardinality "1"^^xsd:nonNegativeInteger
                            ] ,
                            [ rdf:type owl:Restriction ;
                              owl:onProperty :budgetInterval ;
                              owl:cardinality "1"^^xsd:nonNegativeInteger
                            ] ,
                            [ rdf:type owl:Restriction ;
                              owl:onProperty :budgetQuantity ;
                              owl:cardinality "1"^^xsd:nonNegativeInteger
                            ] ;
            rdfs:label "Budget item" .


###  http://linked.data.gov.au/def/auorg#Department
:Department rdf:type owl:Class ;
            rdfs:subClassOf org:OrganizationalUnit ,
                            [ rdf:type owl:Restriction ;
                              owl:onProperty org:purpose ;
                              owl:someValuesFrom :Function
                            ] ,
                            [ rdf:type owl:Restriction ;
                              owl:onProperty org:unitOf ;
                              owl:someValuesFrom :Government
                            ] ;
            rdfs:label "Government Department" .


###  http://linked.data.gov.au/def/auorg#DirectorySubStructure
:DirectorySubStructure rdf:type owl:Class ;
                       rdfs:subClassOf org:OrganizationalUnit ;
                       rdfs:comment "*** Don't understand this one ... ***" ,
                                    "A sub-unit of an Australian government entity"@en ;
                       rdfs:label "Directory sub-structure"@en .


###  http://linked.data.gov.au/def/auorg#Function
:Function rdf:type owl:Class ;
          rdfs:subClassOf <http://www.w3.org/2004/02/skos/core#Concept> ;
          rdfs:label "Government function" .


###  http://linked.data.gov.au/def/auorg#Government
:Government rdf:type owl:Class ;
            rdfs:subClassOf org:FormalOrganization ,
                            [ rdf:type owl:Restriction ;
                              owl:onProperty :levelOfGovernment ;
                              owl:cardinality "1"^^xsd:nonNegativeInteger
                            ] ;
            rdfs:label "Government entity" .


###  http://linked.data.gov.au/def/auorg#NonBoard
:NonBoard rdf:type owl:Class ;
          rdfs:subClassOf org:FormalOrganization ;
          rdfs:comment "An Australian Government non-board entity"@en ;
          rdfs:label "Non-Board"@en .


###  http://linked.data.gov.au/def/auorg#Portfolio
:Portfolio rdf:type owl:Class ;
           rdfs:subClassOf org:Organization ;
           rdfs:comment "A portfolio is a minister's area of responsibility as a member of Cabinet. As a general rule, there is one department in each portfolio."@en ;
           rdfs:label "Portfolio"@en .


###  http://linked.data.gov.au/def/auorg#SingleExecutiveRole
:SingleExecutiveRole rdf:type owl:Class ;
                     rdfs:subClassOf org:Post ;
                     rdfs:comment "A single executive (Senior Executive Service in the Australian Public Service) role"@en ;
                     rdfs:label "Single Executive Role"@en .


###  http://linked.data.gov.au/def/auorg#SumOfMoney
:SumOfMoney rdf:type owl:Class ;
            rdfs:subClassOf [ rdf:type owl:Restriction ;
                              owl:onProperty :moneyAmount ;
                              owl:cardinality "1"^^xsd:nonNegativeInteger
                            ] ,
                            [ rdf:type owl:Restriction ;
                              owl:onProperty :moneyCurrency ;
                              owl:cardinality "1"^^xsd:nonNegativeInteger
                            ] ;
            rdfs:label "Sum of money" .


###  http://www.w3.org/2006/time#ProperInterval
<http://www.w3.org/2006/time#ProperInterval> rdf:type owl:Class .


###  http://www.w3.org/2006/time#TemporalDuration
<http://www.w3.org/2006/time#TemporalDuration> rdf:type owl:Class .


#################################################################
#    Individuals
#################################################################

###  http://linked.data.gov.au/def/auorg#CommonwealthOfAustralia
:CommonwealthOfAustralia rdf:type owl:NamedIndividual ,
                                  :Government ;
                         :levelOfGovernment :Federal ;
                         rdfs:comment "The Australian Government , on behalf of the Commonwealth of Australia"@en ;
                         rdfs:label "Commonwealth of Australia"@en .


###  http://linked.data.gov.au/def/auorg#DepartmentSecretary
:DepartmentSecretary rdf:type owl:NamedIndividual ,
                              org:Role ;
                     rdfs:label "Department Secretary" .


###  http://linked.data.gov.au/def/auorg#Federal
:Federal rdf:type owl:NamedIndividual ,
                  <http://www.w3.org/2004/02/skos/core#Concept> ;
         rdfs:label "Federal" .


###  http://linked.data.gov.au/def/auorg#GovernorGeneral
:GovernorGeneral rdf:type owl:NamedIndividual ,
                          org:Role ;
                 rdfs:comment """The Governor-General of the Commonwealth of Australia, the representative of the Australian monarch.

The Governor-General is appointed by the Australian monarch (also the British monach) on the advice of the Prime Minister of Australia. The Governor-General has formal presidency over the Federal Executive Council and is Commander-in-Chief of the Australian Defence Force"""@en ;
                 rdfs:label "Governor-General"@en .


###  http://linked.data.gov.au/def/auorg#Local
:Local rdf:type owl:NamedIndividual ,
                <http://www.w3.org/2004/02/skos/core#Concept> ;
       rdfs:label "Local government" .


###  http://linked.data.gov.au/def/auorg#Minister
:Minister rdf:type owl:NamedIndividual ,
                   org:Role ;
          rdfs:label "Minister" .


###  http://linked.data.gov.au/def/auorg#State
:State rdf:type owl:NamedIndividual ,
                <http://www.w3.org/2004/02/skos/core#Concept> ;
       rdfs:label "State or Territory" .


###  http://www.w3.org/2006/time#unitYear
<http://www.w3.org/2006/time#unitYear> rdf:type owl:NamedIndividual .


#################################################################
#    Annotations
#################################################################

dc: dct:publisher <http://purl.org/dc/aboutdcmi#DCMI> ;
    dct:title "Dublin Core Metadata Element Set, Version 1.1"@en ;
    dct:modified "2012-06-14"^^xsd:date .


dc:coverage dct:hasVersion <http://dublincore.org/usage/terms/history/#coverage-006> ;
            rdfs:isDefinedBy dc: ;
            dct:modified "2008-01-14"^^xsd:date ;
            <http://www.w3.org/2004/02/skos/core#note> "A second property with the same name as this property has been declared in the dcterms: namespace (http://purl.org/dc/terms/).  See the Introduction to the document \"DCMI Metadata Terms\" (http://dublincore.org/documents/dcmi-terms/) for an explanation."@en ;
            rdfs:comment "The spatial or temporal topic of the resource, the spatial applicability of the resource, or the jurisdiction under which the resource is relevant."@en ;
            dct:description "Spatial topic and spatial applicability may be a named place or a location specified by its geographic coordinates. Temporal topic may be a named period, date, or date range. A jurisdiction may be a named administrative entity or a geographic place to which the resource applies. Recommended best practice is to use a controlled vocabulary such as the Thesaurus of Geographic Names [TGN]. Where appropriate, named places or time periods can be used in preference to numeric identifiers such as sets of coordinates or date ranges."@en ;
            dct:issued "1999-07-02"^^xsd:date ;
            rdfs:label "Coverage"@en .


dc:date dct:issued "1999-07-02"^^xsd:date ;
        <http://www.w3.org/2004/02/skos/core#note> "A second property with the same name as this property has been declared in the dcterms: namespace (http://purl.org/dc/terms/).  See the Introduction to the document \"DCMI Metadata Terms\" (http://dublincore.org/documents/dcmi-terms/) for an explanation."@en ;
        dct:modified "2008-01-14"^^xsd:date ;
        rdfs:isDefinedBy dc: ;
        dct:hasVersion <http://dublincore.org/usage/terms/history/#date-006> ;
        rdfs:comment "A point or period of time associated with an event in the lifecycle of the resource."@en ;
        dct:description "Date may be used to express temporal information at any level of granularity.  Recommended best practice is to use an encoding scheme, such as the W3CDTF profile of ISO 8601 [W3CDTF]."@en ;
        rdfs:label "Date"@en .


dc:description dct:description "Description may include but is not limited to: an abstract, a table of contents, a graphical representation, or a free-text account of the resource."@en ;
               rdfs:isDefinedBy dc: ;
               dct:issued "1999-07-02"^^xsd:date ;
               <http://www.w3.org/2004/02/skos/core#note> "A second property with the same name as this property has been declared in the dcterms: namespace (http://purl.org/dc/terms/).  See the Introduction to the document \"DCMI Metadata Terms\" (http://dublincore.org/documents/dcmi-terms/) for an explanation."@en ;
               rdfs:comment "An account of the resource."@en ;
               dct:modified "2008-01-14"^^xsd:date ;
               rdfs:label "Description"@en ;
               dct:hasVersion <http://dublincore.org/usage/terms/history/#description-006> .


dc:format <http://www.w3.org/2004/02/skos/core#note> "A second property with the same name as this property has been declared in the dcterms: namespace (http://purl.org/dc/terms/).  See the Introduction to the document \"DCMI Metadata Terms\" (http://dublincore.org/documents/dcmi-terms/) for an explanation."@en ;
          dct:issued "1999-07-02"^^xsd:date ;
          dct:modified "2008-01-14"^^xsd:date ;
          rdfs:label "Format"@en ;
          rdfs:comment "The file format, physical medium, or dimensions of the resource."@en ;
          dct:hasVersion <http://dublincore.org/usage/terms/history/#format-007> ;
          rdfs:isDefinedBy dc: ;
          dct:description "Examples of dimensions include size and duration. Recommended best practice is to use a controlled vocabulary such as the list of Internet Media Types [MIME]."@en .


dc:identifier dct:hasVersion <http://dublincore.org/usage/terms/history/#identifier-006> ;
              rdfs:isDefinedBy dc: ;
              dct:description "Recommended best practice is to identify the resource by means of a string conforming to a formal identification system. "@en ;
              rdfs:comment "An unambiguous reference to the resource within a given context."@en ;
              dct:issued "1999-07-02"^^xsd:date ;
              dct:modified "2008-01-14"^^xsd:date ;
              rdfs:label "Identifier"@en ;
              <http://www.w3.org/2004/02/skos/core#note> "A second property with the same name as this property has been declared in the dcterms: namespace (http://purl.org/dc/terms/).  See the Introduction to the document \"DCMI Metadata Terms\" (http://dublincore.org/documents/dcmi-terms/) for an explanation."@en .


dc:language dct:modified "2008-01-14"^^xsd:date ;
            dct:issued "1999-07-02"^^xsd:date ;
            <http://www.w3.org/2004/02/skos/core#note> "A second property with the same name as this property has been declared in the dcterms: namespace (http://purl.org/dc/terms/).  See the Introduction to the document \"DCMI Metadata Terms\" (http://dublincore.org/documents/dcmi-terms/) for an explanation."@en ;
            dct:hasVersion <http://dublincore.org/usage/terms/history/#language-007> ;
            rdfs:label "Language"@en ;
            dct:description "Recommended best practice is to use a controlled vocabulary such as RFC 4646 [RFC4646]."@en ;
            rdfs:isDefinedBy dc: ;
            rdfs:comment "A language of the resource."@en ;
            rdfs:seeAlso <http://www.ietf.org/rfc/rfc4646.txt> .


dc:relation dct:hasVersion <http://dublincore.org/usage/terms/history/#relation-006> ;
            dct:description "Recommended best practice is to identify the related resource by means of a string conforming to a formal identification system. "@en ;
            rdfs:label "Relation"@en ;
            dct:modified "2008-01-14"^^xsd:date ;
            dct:issued "1999-07-02"^^xsd:date ;
            <http://www.w3.org/2004/02/skos/core#note> "A second property with the same name as this property has been declared in the dcterms: namespace (http://purl.org/dc/terms/).  See the Introduction to the document \"DCMI Metadata Terms\" (http://dublincore.org/documents/dcmi-terms/) for an explanation."@en ;
            rdfs:comment "A related resource."@en ;
            rdfs:isDefinedBy dc: .


dc:rights dct:hasVersion <http://dublincore.org/usage/terms/history/#rights-006> ;
          rdfs:isDefinedBy dc: ;
          <http://www.w3.org/2004/02/skos/core#note> "A second property with the same name as this property has been declared in the dcterms: namespace (http://purl.org/dc/terms/).  See the Introduction to the document \"DCMI Metadata Terms\" (http://dublincore.org/documents/dcmi-terms/) for an explanation."@en ;
          dct:issued "1999-07-02"^^xsd:date ;
          dct:description "Typically, rights information includes a statement about various property rights associated with the resource, including intellectual property rights."@en ;
          rdfs:label "Rights"@en ;
          dct:modified "2008-01-14"^^xsd:date ;
          rdfs:comment "Information about rights held in and over the resource."@en .


dc:source dct:hasVersion <http://dublincore.org/usage/terms/history/#source-006> ;
          <http://www.w3.org/2004/02/skos/core#note> "A second property with the same name as this property has been declared in the dcterms: namespace (http://purl.org/dc/terms/).  See the Introduction to the document \"DCMI Metadata Terms\" (http://dublincore.org/documents/dcmi-terms/) for an explanation."@en ;
          rdfs:isDefinedBy dc: ;
          rdfs:comment "A related resource from which the described resource is derived."@en ;
          dct:modified "2008-01-14"^^xsd:date ;
          dct:issued "1999-07-02"^^xsd:date ;
          dct:description "The described resource may be derived from the related resource in whole or in part. Recommended best practice is to identify the related resource by means of a string conforming to a formal identification system."@en ;
          rdfs:label "Source"@en .


dc:subject dct:description "Typically, the subject will be represented using keywords, key phrases, or classification codes. Recommended best practice is to use a controlled vocabulary."@en ;
           <http://www.w3.org/2004/02/skos/core#note> "A second property with the same name as this property has been declared in the dcterms: namespace (http://purl.org/dc/terms/).  See the Introduction to the document \"DCMI Metadata Terms\" (http://dublincore.org/documents/dcmi-terms/) for an explanation."@en ;
           dct:issued "1999-07-02"^^xsd:date ;
           rdfs:label "Subject"@en ;
           rdfs:comment "The topic of the resource."@en ;
           rdfs:isDefinedBy dc: ;
           dct:modified "2012-06-14"^^xsd:date ;
           dct:hasVersion <http://dublincore.org/usage/terms/history/#subject-007> .


dc:title rdfs:comment "A name given to the resource."@en ;
         dct:modified "2008-01-14"^^xsd:date ;
         <http://www.w3.org/2004/02/skos/core#note> "A second property with the same name as this property has been declared in the dcterms: namespace (http://purl.org/dc/terms/).  See the Introduction to the document \"DCMI Metadata Terms\" (http://dublincore.org/documents/dcmi-terms/) for an explanation."@en ;
         rdfs:label "Title"@en ;
         dct:issued "1999-07-02"^^xsd:date ;
         dct:hasVersion <http://dublincore.org/usage/terms/history/#title-006> ;
         rdfs:isDefinedBy dc: .


dc:type rdfs:comment "The nature or genre of the resource."@en ;
        dct:hasVersion <http://dublincore.org/usage/terms/history/#type-006> ;
        rdfs:label "Type"@en ;
        rdfs:isDefinedBy dc: ;
        dct:description "Recommended best practice is to use a controlled vocabulary such as the DCMI Type Vocabulary [DCMITYPE]. To describe the file format, physical medium, or dimensions of the resource, use the Format element."@en ;
        dct:issued "1999-07-02"^^xsd:date ;
        <http://www.w3.org/2004/02/skos/core#note> "A second property with the same name as this property has been declared in the dcterms: namespace (http://purl.org/dc/terms/).  See the Introduction to the document \"DCMI Metadata Terms\" (http://dublincore.org/documents/dcmi-terms/) for an explanation."@en ;
        dct:modified "2008-01-14"^^xsd:date .


###  Generated by the OWL API (version 4.2.8.20170104-2310) https://github.com/owlcs/owlapi
