# baseURI: http://test.linked.data.gov.au/def/auorg
# imports: http://purl.org/dc/elements/1.1/
# imports: http://www.w3.org/2006/time
# imports: http://www.w3.org/ns/org#
# imports: http://www.w3.org/ns/time/gregorian

@prefix : <http://test.linked.data.gov.au/def/auorg#> .
@prefix dct: <http://purl.org/dc/terms/> .
@prefix gnaf: <http://gnafld.net/def/gnaf#> .
@prefix org: <http://www.w3.org/ns/org#> .
@prefix owl: <http://www.w3.org/2002/07/owl#> .
@prefix rdf: <http://www.w3.org/1999/02/22-rdf-syntax-ns#> .
@prefix rdfs: <http://www.w3.org/2000/01/rdf-schema#> .
@prefix skos: <http://www.w3.org/2004/02/skos/core#> .
@prefix xml: <http://www.w3.org/XML/1998/namespace> .
@prefix xsd: <http://www.w3.org/2001/XMLSchema#> .

gnaf:Address
  rdf:type owl:Class ;
  rdfs:comment "An Address object, defined by the GNAF ontology and supplied by the GNAF dataset only."@en ;
  rdfs:label "Address"@en ;
  rdfs:subClassOf org:Site ;
.
<http://purl.org/dc/elements/1.1/>
  dct:modified "2012-06-14"^^xsd:date ;
  dct:publisher <http://purl.org/dc/aboutdcmi#DCMI> ;
  dct:title "Dublin Core Metadata Element Set, Version 1.1"@en ;
.
<http://purl.org/dc/elements/1.1/contributor>
  dct:description "Examples of a Contributor include a person, an organization, or a service. Typically, the name of a Contributor should be used to indicate the entity."@en ;
  dct:hasVersion <http://dublincore.org/usage/terms/history/#contributor-006> ;
  dct:issued "1999-07-02"^^xsd:date ;
  dct:modified "2008-01-14"^^xsd:date ;
  rdfs:comment "An entity responsible for making contributions to the resource."@en ;
  rdfs:isDefinedBy <http://purl.org/dc/elements/1.1/> ;
  rdfs:label "Contributor"@en ;
  skos:note "A second property with the same name as this property has been declared in the dcterms: namespace (http://purl.org/dc/terms/).  See the Introduction to the document \"DCMI Metadata Terms\" (http://dublincore.org/documents/dcmi-terms/) for an explanation."@en ;
.
<http://purl.org/dc/elements/1.1/coverage>
  dct:description "Spatial topic and spatial applicability may be a named place or a location specified by its geographic coordinates. Temporal topic may be a named period, date, or date range. A jurisdiction may be a named administrative entity or a geographic place to which the resource applies. Recommended best practice is to use a controlled vocabulary such as the Thesaurus of Geographic Names [TGN]. Where appropriate, named places or time periods can be used in preference to numeric identifiers such as sets of coordinates or date ranges."@en ;
  dct:hasVersion <http://dublincore.org/usage/terms/history/#coverage-006> ;
  dct:issued "1999-07-02"^^xsd:date ;
  dct:modified "2008-01-14"^^xsd:date ;
  rdfs:comment "The spatial or temporal topic of the resource, the spatial applicability of the resource, or the jurisdiction under which the resource is relevant."@en ;
  rdfs:isDefinedBy <http://purl.org/dc/elements/1.1/> ;
  rdfs:label "Coverage"@en ;
  skos:note "A second property with the same name as this property has been declared in the dcterms: namespace (http://purl.org/dc/terms/).  See the Introduction to the document \"DCMI Metadata Terms\" (http://dublincore.org/documents/dcmi-terms/) for an explanation."@en ;
.
<http://purl.org/dc/elements/1.1/creator>
  dct:description "Examples of a Creator include a person, an organization, or a service. Typically, the name of a Creator should be used to indicate the entity."@en ;
  dct:hasVersion <http://dublincore.org/usage/terms/history/#creator-006> ;
  dct:issued "1999-07-02"^^xsd:date ;
  dct:modified "2008-01-14"^^xsd:date ;
  rdfs:comment "An entity primarily responsible for making the resource."@en ;
  rdfs:isDefinedBy <http://purl.org/dc/elements/1.1/> ;
  rdfs:label "Creator"@en ;
  skos:note "A second property with the same name as this property has been declared in the dcterms: namespace (http://purl.org/dc/terms/).  See the Introduction to the document \"DCMI Metadata Terms\" (http://dublincore.org/documents/dcmi-terms/) for an explanation."@en ;
.
<http://purl.org/dc/elements/1.1/date>
  dct:description "Date may be used to express temporal information at any level of granularity.  Recommended best practice is to use an encoding scheme, such as the W3CDTF profile of ISO 8601 [W3CDTF]."@en ;
  dct:hasVersion <http://dublincore.org/usage/terms/history/#date-006> ;
  dct:issued "1999-07-02"^^xsd:date ;
  dct:modified "2008-01-14"^^xsd:date ;
  rdfs:comment "A point or period of time associated with an event in the lifecycle of the resource."@en ;
  rdfs:isDefinedBy <http://purl.org/dc/elements/1.1/> ;
  rdfs:label "Date"@en ;
  skos:note "A second property with the same name as this property has been declared in the dcterms: namespace (http://purl.org/dc/terms/).  See the Introduction to the document \"DCMI Metadata Terms\" (http://dublincore.org/documents/dcmi-terms/) for an explanation."@en ;
.
<http://purl.org/dc/elements/1.1/description>
  dct:description "Description may include but is not limited to: an abstract, a table of contents, a graphical representation, or a free-text account of the resource."@en ;
  dct:hasVersion <http://dublincore.org/usage/terms/history/#description-006> ;
  dct:issued "1999-07-02"^^xsd:date ;
  dct:modified "2008-01-14"^^xsd:date ;
  rdfs:comment "An account of the resource."@en ;
  rdfs:isDefinedBy <http://purl.org/dc/elements/1.1/> ;
  rdfs:label "Description"@en ;
  skos:note "A second property with the same name as this property has been declared in the dcterms: namespace (http://purl.org/dc/terms/).  See the Introduction to the document \"DCMI Metadata Terms\" (http://dublincore.org/documents/dcmi-terms/) for an explanation."@en ;
.
<http://purl.org/dc/elements/1.1/format>
  dct:description "Examples of dimensions include size and duration. Recommended best practice is to use a controlled vocabulary such as the list of Internet Media Types [MIME]."@en ;
  dct:hasVersion <http://dublincore.org/usage/terms/history/#format-007> ;
  dct:issued "1999-07-02"^^xsd:date ;
  dct:modified "2008-01-14"^^xsd:date ;
  rdfs:comment "The file format, physical medium, or dimensions of the resource."@en ;
  rdfs:isDefinedBy <http://purl.org/dc/elements/1.1/> ;
  rdfs:label "Format"@en ;
  skos:note "A second property with the same name as this property has been declared in the dcterms: namespace (http://purl.org/dc/terms/).  See the Introduction to the document \"DCMI Metadata Terms\" (http://dublincore.org/documents/dcmi-terms/) for an explanation."@en ;
.
<http://purl.org/dc/elements/1.1/identifier>
  dct:description "Recommended best practice is to identify the resource by means of a string conforming to a formal identification system. "@en ;
  dct:hasVersion <http://dublincore.org/usage/terms/history/#identifier-006> ;
  dct:issued "1999-07-02"^^xsd:date ;
  dct:modified "2008-01-14"^^xsd:date ;
  rdfs:comment "An unambiguous reference to the resource within a given context."@en ;
  rdfs:isDefinedBy <http://purl.org/dc/elements/1.1/> ;
  rdfs:label "Identifier"@en ;
  skos:note "A second property with the same name as this property has been declared in the dcterms: namespace (http://purl.org/dc/terms/).  See the Introduction to the document \"DCMI Metadata Terms\" (http://dublincore.org/documents/dcmi-terms/) for an explanation."@en ;
.
<http://purl.org/dc/elements/1.1/language>
  dct:description "Recommended best practice is to use a controlled vocabulary such as RFC 4646 [RFC4646]."@en ;
  dct:hasVersion <http://dublincore.org/usage/terms/history/#language-007> ;
  dct:issued "1999-07-02"^^xsd:date ;
  dct:modified "2008-01-14"^^xsd:date ;
  rdfs:comment "A language of the resource."@en ;
  rdfs:isDefinedBy <http://purl.org/dc/elements/1.1/> ;
  rdfs:label "Language"@en ;
  rdfs:seeAlso <http://www.ietf.org/rfc/rfc4646.txt> ;
  skos:note "A second property with the same name as this property has been declared in the dcterms: namespace (http://purl.org/dc/terms/).  See the Introduction to the document \"DCMI Metadata Terms\" (http://dublincore.org/documents/dcmi-terms/) for an explanation."@en ;
.
<http://purl.org/dc/elements/1.1/publisher>
  dct:description "Examples of a Publisher include a person, an organization, or a service. Typically, the name of a Publisher should be used to indicate the entity."@en ;
  dct:hasVersion <http://dublincore.org/usage/terms/history/#publisher-006> ;
  dct:issued "1999-07-02"^^xsd:date ;
  dct:modified "2008-01-14"^^xsd:date ;
  rdfs:comment "An entity responsible for making the resource available."@en ;
  rdfs:isDefinedBy <http://purl.org/dc/elements/1.1/> ;
  rdfs:label "Publisher"@en ;
  skos:note "A second property with the same name as this property has been declared in the dcterms: namespace (http://purl.org/dc/terms/).  See the Introduction to the document \"DCMI Metadata Terms\" (http://dublincore.org/documents/dcmi-terms/) for an explanation."@en ;
.
<http://purl.org/dc/elements/1.1/relation>
  dct:description "Recommended best practice is to identify the related resource by means of a string conforming to a formal identification system. "@en ;
  dct:hasVersion <http://dublincore.org/usage/terms/history/#relation-006> ;
  dct:issued "1999-07-02"^^xsd:date ;
  dct:modified "2008-01-14"^^xsd:date ;
  rdfs:comment "A related resource."@en ;
  rdfs:isDefinedBy <http://purl.org/dc/elements/1.1/> ;
  rdfs:label "Relation"@en ;
  skos:note "A second property with the same name as this property has been declared in the dcterms: namespace (http://purl.org/dc/terms/).  See the Introduction to the document \"DCMI Metadata Terms\" (http://dublincore.org/documents/dcmi-terms/) for an explanation."@en ;
.
<http://purl.org/dc/elements/1.1/rights>
  dct:description "Typically, rights information includes a statement about various property rights associated with the resource, including intellectual property rights."@en ;
  dct:hasVersion <http://dublincore.org/usage/terms/history/#rights-006> ;
  dct:issued "1999-07-02"^^xsd:date ;
  dct:modified "2008-01-14"^^xsd:date ;
  rdfs:comment "Information about rights held in and over the resource."@en ;
  rdfs:isDefinedBy <http://purl.org/dc/elements/1.1/> ;
  rdfs:label "Rights"@en ;
  skos:note "A second property with the same name as this property has been declared in the dcterms: namespace (http://purl.org/dc/terms/).  See the Introduction to the document \"DCMI Metadata Terms\" (http://dublincore.org/documents/dcmi-terms/) for an explanation."@en ;
.
<http://purl.org/dc/elements/1.1/source>
  dct:description "The described resource may be derived from the related resource in whole or in part. Recommended best practice is to identify the related resource by means of a string conforming to a formal identification system."@en ;
  dct:hasVersion <http://dublincore.org/usage/terms/history/#source-006> ;
  dct:issued "1999-07-02"^^xsd:date ;
  dct:modified "2008-01-14"^^xsd:date ;
  rdfs:comment "A related resource from which the described resource is derived."@en ;
  rdfs:isDefinedBy <http://purl.org/dc/elements/1.1/> ;
  rdfs:label "Source"@en ;
  skos:note "A second property with the same name as this property has been declared in the dcterms: namespace (http://purl.org/dc/terms/).  See the Introduction to the document \"DCMI Metadata Terms\" (http://dublincore.org/documents/dcmi-terms/) for an explanation."@en ;
.
<http://purl.org/dc/elements/1.1/subject>
  dct:description "Typically, the subject will be represented using keywords, key phrases, or classification codes. Recommended best practice is to use a controlled vocabulary."@en ;
  dct:hasVersion <http://dublincore.org/usage/terms/history/#subject-007> ;
  dct:issued "1999-07-02"^^xsd:date ;
  dct:modified "2012-06-14"^^xsd:date ;
  rdfs:comment "The topic of the resource."@en ;
  rdfs:isDefinedBy <http://purl.org/dc/elements/1.1/> ;
  rdfs:label "Subject"@en ;
  skos:note "A second property with the same name as this property has been declared in the dcterms: namespace (http://purl.org/dc/terms/).  See the Introduction to the document \"DCMI Metadata Terms\" (http://dublincore.org/documents/dcmi-terms/) for an explanation."@en ;
.
<http://purl.org/dc/elements/1.1/title>
  dct:hasVersion <http://dublincore.org/usage/terms/history/#title-006> ;
  dct:issued "1999-07-02"^^xsd:date ;
  dct:modified "2008-01-14"^^xsd:date ;
  rdfs:comment "A name given to the resource."@en ;
  rdfs:isDefinedBy <http://purl.org/dc/elements/1.1/> ;
  rdfs:label "Title"@en ;
  skos:note "A second property with the same name as this property has been declared in the dcterms: namespace (http://purl.org/dc/terms/).  See the Introduction to the document \"DCMI Metadata Terms\" (http://dublincore.org/documents/dcmi-terms/) for an explanation."@en ;
.
<http://purl.org/dc/elements/1.1/type>
  dct:description "Recommended best practice is to use a controlled vocabulary such as the DCMI Type Vocabulary [DCMITYPE]. To describe the file format, physical medium, or dimensions of the resource, use the Format element."@en ;
  dct:hasVersion <http://dublincore.org/usage/terms/history/#type-006> ;
  dct:issued "1999-07-02"^^xsd:date ;
  dct:modified "2008-01-14"^^xsd:date ;
  rdfs:comment "The nature or genre of the resource."@en ;
  rdfs:isDefinedBy <http://purl.org/dc/elements/1.1/> ;
  rdfs:label "Type"@en ;
  skos:note "A second property with the same name as this property has been declared in the dcterms: namespace (http://purl.org/dc/terms/).  See the Introduction to the document \"DCMI Metadata Terms\" (http://dublincore.org/documents/dcmi-terms/) for an explanation."@en ;
.
dct:description
  rdf:type owl:AnnotationProperty ;
.
dct:hasVersion
  rdf:type owl:AnnotationProperty ;
.
dct:issued
  rdf:type owl:AnnotationProperty ;
.
dct:modified
  rdf:type owl:AnnotationProperty ;
.
dct:publisher
  rdf:type owl:AnnotationProperty ;
.
dct:title
  rdf:type owl:AnnotationProperty ;
.
<http://test.linked.data.gov.au/def/auorg>
  rdf:type owl:Ontology ;
  dct:contributor <https://orcid.org/0000-0002-3884-3420> ;
  dct:created "2018-05-21"^^xsd:date ;
  dct:creator <http://orcid.org/0000-0002-8742-7730> ;
  dct:creator "Nicholas Car" ;
  dct:modified "2012-06-14"^^xsd:date ;
  dct:modified "2018-05-21"^^xsd:date ;
  dct:publisher <http://purl.org/dc/aboutdcmi#DCMI> ;
  dct:title "Dublin Core Metadata Element Set, Version 1.1"@en ;
  rdfs:comment """This ontology defines a series of sub classes of the generic org:Organization class to describe types of Australian Government organisations represented in the website directory.data.gov.au. It also defines a series of properties for organisations to capture specific properties of those organisations also given in directory.gov.au.

This ontology is incomplete as of v0.5 and is currently for demo purposes only."""@en ;
  rdfs:label "AU Org Ontology"@en ;
  rdfs:seeAlso "The GitHub repository containing addition documentation: http://github.com/CSIRO-enviro-informatics/auorg-ont/"@en ;
  owl:imports <http://purl.org/dc/elements/1.1/> ;
  owl:imports <http://www.w3.org/2006/time> ;
  owl:imports org: ;
  owl:imports <http://www.w3.org/ns/time/gregorian> ;
  owl:versionIRI <http://test.linked.data.gov.au/def/auorg/0.5> ;
  owl:versionInfo "Beta version"@en ;
.
:Agency
  rdf:type owl:Class ;
  rdfs:label "Government Agency" ;
  rdfs:subClassOf :Entity ;
  rdfs:subClassOf [
      rdf:type owl:Restriction ;
      owl:onProperty org:linkedTo ;
      owl:someValuesFrom :Jurisdiction ;
    ] ;
  rdfs:subClassOf [
      rdf:type owl:Restriction ;
      owl:onProperty org:purpose ;
      owl:someValuesFrom :Function ;
    ] ;
.
:Appropriations
  rdf:type owl:Class ;
  rdfs:label "Appropriations budget (annualized)" ;
  rdfs:subClassOf :BudgetItem ;
  rdfs:subClassOf [
      rdf:type owl:Restriction ;
      owl:allValuesFrom :AustralianDollars ;
      owl:onProperty :budgetQuantity ;
    ] ;
  rdfs:subClassOf [
      rdf:type owl:Restriction ;
      owl:hasValue :CommonwealthOfAustralia ;
      owl:onProperty :budgetSource ;
    ] ;
  rdfs:subClassOf [
      rdf:type owl:Restriction ;
      owl:hasValue <http://www.w3.org/2006/time#unitYear> ;
      owl:onProperty :budgetDuration ;
    ] ;
.
:AustralianDollars
  rdf:type owl:Class ;
  rdfs:comment "Sum of money in whole Australian Dollars"@en ;
  rdfs:label "Australian Dollars"@en ;
  rdfs:subClassOf :SumOfMoney ;
  rdfs:subClassOf [
      rdf:type owl:Restriction ;
      owl:allValuesFrom xsd:integer ;
      owl:onProperty :moneyAmount ;
    ] ;
  rdfs:subClassOf [
      rdf:type owl:Restriction ;
      owl:hasValue "AUD" ;
      owl:onProperty :moneyCurrency ;
    ] ;
.
:Board
  rdf:type owl:Class ;
  rdfs:comment "An Australian Government Board"@en ;
  rdfs:label "Board"@en ;
  rdfs:subClassOf org:FormalOrganization ;
.
:BudgetItem
  rdf:type owl:Class ;
  rdfs:label "Budget item" ;
  rdfs:subClassOf [
      rdf:type owl:Restriction ;
      owl:cardinality "1"^^xsd:nonNegativeInteger ;
      owl:onProperty :budgetDuration ;
    ] ;
  rdfs:subClassOf [
      rdf:type owl:Restriction ;
      owl:cardinality "1"^^xsd:nonNegativeInteger ;
      owl:onProperty :budgetInterval ;
    ] ;
  rdfs:subClassOf [
      rdf:type owl:Restriction ;
      owl:cardinality "1"^^xsd:nonNegativeInteger ;
      owl:onProperty :budgetQuantity ;
    ] ;
  rdfs:subClassOf [
      rdf:type owl:Restriction ;
      owl:minCardinality "1"^^xsd:nonNegativeInteger ;
      owl:onProperty :budgetPurpose ;
    ] ;
  rdfs:subClassOf [
      rdf:type owl:Restriction ;
      owl:minCardinality "1"^^xsd:nonNegativeInteger ;
      owl:onProperty :budgetSource ;
    ] ;
.
:CommonwealthOfAustralia
  rdf:type :Jurisdiction ;
  rdf:type owl:NamedIndividual ;
  :levelOfGovernment :Federal ;
  rdfs:comment "The Australian Government , on behalf of the Commonwealth of Australia"@en ;
  rdfs:label "Commonwealth of Australia"@en ;
.
:Department
  rdf:type owl:Class ;
  rdfs:label "Government Department" ;
  rdfs:subClassOf :Entity ;
  rdfs:subClassOf org:OrganizationalUnit ;
  rdfs:subClassOf [
      rdf:type owl:Restriction ;
      owl:onProperty org:purpose ;
      owl:someValuesFrom :Function ;
    ] ;
  rdfs:subClassOf [
      rdf:type owl:Restriction ;
      owl:onProperty org:unitOf ;
      owl:someValuesFrom :Jurisdiction ;
    ] ;
.
:DepartmentSecretary
  rdf:type owl:NamedIndividual ;
  rdf:type org:Role ;
  rdfs:label "Department Secretary" ;
.
:DirectorySubStructure
  rdf:type owl:Class ;
  rdfs:comment "*** Don't understand this one ... ***" ;
  rdfs:comment "A sub-unit of an Australian government entity"@en ;
  rdfs:label "Directory sub-structure"@en ;
  rdfs:subClassOf org:OrganizationalUnit ;
.
:Entity
  rdf:type owl:Class ;
  rdfs:comment "Government entity, any kind, any level of government" ;
  rdfs:label "Government Entity" ;
  rdfs:subClassOf org:Organization ;
  rdfs:subClassOf [
      rdf:type owl:Restriction ;
      owl:cardinality "1"^^xsd:nonNegativeInteger ;
      owl:onProperty :levelOfGovernment ;
    ] ;
.
:Federal
  rdf:type owl:NamedIndividual ;
  rdf:type skos:Concept ;
  rdfs:label "Federal" ;
.
:Function
  rdf:type owl:Class ;
  rdfs:label "Government function" ;
  rdfs:subClassOf skos:Concept ;
.
:GovernorGeneral
  rdf:type owl:NamedIndividual ;
  rdf:type org:Role ;
  rdfs:comment """The Governor-General of the Commonwealth of Australia, the representative of the Australian monarch.

The Governor-General is appointed by the Australian monarch (also the British monach) on the advice of the Prime Minister of Australia. The Governor-General has formal presidency over the Federal Executive Council and is Commander-in-Chief of the Australian Defence Force"""@en ;
  rdfs:label "Governor-General"@en ;
.
:Jurisdiction
  rdf:type owl:Class ;
  rdfs:comment "This applies to the top/autonomous government entity - e.g. one for each national, state, local government jurisdiction" ;
  rdfs:label "Government or Jurisdiction" ;
  rdfs:subClassOf :Entity ;
  rdfs:subClassOf org:FormalOrganization ;
.
:Local
  rdf:type owl:NamedIndividual ;
  rdf:type skos:Concept ;
  rdfs:label "Local government" ;
.
:Minister
  rdf:type owl:NamedIndividual ;
  rdf:type org:Role ;
  rdfs:label "Minister" ;
.
:NonBoard
  rdf:type owl:Class ;
  rdfs:comment "An Australian Government non-board entity"@en ;
  rdfs:label "Non-Board"@en ;
  rdfs:subClassOf org:FormalOrganization ;
.
:Outcome
  rdf:type owl:Class ;
  rdfs:label "Government Outcome" ;
  rdfs:subClassOf :Function ;
.
:Portfolio
  rdf:type owl:Class ;
  rdfs:comment "A portfolio is a minister's area of responsibility as a member of Cabinet. As a general rule, there is one department associated with each portfolio."@en ;
  rdfs:comment "Is this an organization or is this a classifier?" ;
  rdfs:label "Government Portfolio"@en ;
  rdfs:subClassOf :Function ;
.
:Program
  rdf:type owl:Class ;
  rdfs:label "Government Program" ;
  rdfs:subClassOf :Function ;
.
:SingleExecutiveRole
  rdf:type owl:Class ;
  rdfs:comment "A single executive (Senior Executive Service in the Australian Public Service) role"@en ;
  rdfs:label "Single Executive Role"@en ;
  rdfs:subClassOf org:Post ;
.
:State
  rdf:type owl:NamedIndividual ;
  rdf:type skos:Concept ;
  rdfs:label "State or Territory" ;
.
:SumOfMoney
  rdf:type owl:Class ;
  rdfs:label "Sum of money" ;
  rdfs:subClassOf [
      rdf:type owl:Restriction ;
      owl:cardinality "1"^^xsd:nonNegativeInteger ;
      owl:onProperty :moneyAmount ;
    ] ;
  rdfs:subClassOf [
      rdf:type owl:Restriction ;
      owl:cardinality "1"^^xsd:nonNegativeInteger ;
      owl:onProperty :moneyCurrency ;
    ] ;
.
:budgetDuration
  rdf:type owl:ObjectProperty ;
  rdfs:domain :BudgetItem ;
  rdfs:label "duration of interval over which budget applies" ;
  rdfs:range <http://www.w3.org/2006/time#TemporalDuration> ;
.
:budgetInterval
  rdf:type owl:ObjectProperty ;
  rdfs:domain :BudgetItem ;
  rdfs:label "interval over which budget applies" ;
  rdfs:range <http://www.w3.org/2006/time#ProperInterval> ;
.
:budgetPurpose
  rdf:type owl:ObjectProperty ;
  rdfs:domain :BudgetItem ;
  rdfs:label "purpose for which budget is allocated" ;
  rdfs:range :Function ;
.
:budgetQuantity
  rdf:type owl:ObjectProperty ;
  rdfs:domain :BudgetItem ;
  rdfs:label "budget quantity" ;
  rdfs:range :SumOfMoney ;
.
:budgetSource
  rdf:type owl:ObjectProperty ;
  rdfs:domain :BudgetItem ;
  rdfs:label "source of budget" ;
  rdfs:range <http://xmlns.com/foaf/0.1/Agent> ;
.
:hasABN
  rdf:type owl:DatatypeProperty ;
  rdfs:comment "org:identifier is a sub-property of skos:notation, which is a owl:DatatypeProperty, i.e. a literal. Could be constrained to be a string with the pattern 'NN NNN NNN NNN` to match ABN structure" ;
  rdfs:range xsd:integer ;
  rdfs:subPropertyOf org:identifier ;
.
:hasAppropriations
  rdf:type owl:ObjectProperty ;
  rdfs:comment "Has a current annual budgetary appropriation amount in Australian Dollars" ;
  rdfs:label "Annual appropriation budget (AUD)" ;
  rdfs:range :Appropriations ;
  rdfs:subPropertyOf :hasBudgetItem ;
.
:hasAverageStaffingLevel
  rdf:type owl:DatatypeProperty ;
  rdfs:comment "Has an average annual staffig level of (no. of people)"@en ;
  rdfs:label "has average staffing level"@en ;
  rdfs:range xsd:integer ;
.
:hasBudgetItem
  rdf:type owl:ObjectProperty ;
  rdfs:domain org:Organization ;
  rdfs:label "budget item" ;
  rdfs:range :BudgetItem ;
.
:hasStreetAddress
  rdf:type owl:ObjectProperty ;
  rdfs:comment "Has a GNAF address of"@en ;
  rdfs:label "has street address"@en ;
  rdfs:range gnaf:Address ;
  rdfs:subPropertyOf org:hasSite ;
.
:inPortfolio
  rdf:type owl:ObjectProperty ;
  rdfs:comment "is within a particular government Portfolio"@en ;
  rdfs:label "in portfolio"@en ;
  rdfs:range :Portfolio ;
  rdfs:subPropertyOf org:subOrganizationOf ;
.
:levelOfGovernment
  rdf:type owl:ObjectProperty ;
  rdfs:domain :Jurisdiction ;
  rdfs:label "level of government (Federal, State, Local)" ;
  rdfs:subPropertyOf org:classification ;
.
:moneyAmount
  rdf:type owl:DatatypeProperty ;
  rdfs:domain :SumOfMoney ;
  rdfs:label "Money amount" ;
  rdfs:range xsd:decimal ;
.
:moneyCurrency
  rdf:type owl:DatatypeProperty ;
  rdfs:domain :SumOfMoney ;
  rdfs:label "Money currency - ISO 4217 code" ;
  rdfs:range xsd:string ;
.
xsd:date
  rdf:type rdfs:Datatype ;
.
skos:note
  rdf:type owl:AnnotationProperty ;
.
<http://www.w3.org/2006/time#ProperInterval>
  rdf:type owl:Class ;
.
<http://www.w3.org/2006/time#TemporalDuration>
  rdf:type owl:Class ;
.
<http://www.w3.org/2006/time#unitYear>
  rdf:type owl:NamedIndividual ;
.
org:purpose
  rdf:type owl:ObjectProperty ;
.
